Surface/Term/Substitution.lean
@@ -4,200 +4,206 @@ import Surface.Ty
 
 open LeanSubst
 
+namespace Surface
+
 @[coe]
-def Surface.Term.from_action : Subst.Action Surface.Term -> Surface.Term
+def Term.from_action : Subst.Action Term -> Term
 | .re y => `#y
 | .su t => t
 
 @[simp]
-theorem Surface.Term.from_action_id {n} : from_action (+0 n) = `#n := by
+theorem Term.from_action_id {n} : from_action (+0 n) = `#n := by
   simp [from_action, Subst.id]
 
 @[simp]
-theorem Surface.Term.from_action_succ {n} : from_action (+1 n) = `#(n + 1) := by
+theorem Term.from_action_succ {n} : from_action (+1 n) = `#(n + 1) := by
   simp [from_action, Subst.succ]
 
 @[simp]
-theorem Surface.Term.from_acton_re {n} : from_action (re n) = `#n := by simp [from_action]
+theorem Term.from_acton_re {n} : from_action (re n) = `#n := by simp [from_action]
 
 @[simp]
-theorem Surface.Term.from_action_su {t} : from_action (su t) = t := by simp [from_action]
+theorem Term.from_action_su {t} : from_action (su t) = t := by simp [from_action]
 
-instance Surface.instCoe_ActionTermTerm : Coe (Subst.Action Surface.Term) Surface.Term where
-  coe := Surface.Term.from_action
+instance instCoe_ActionTermTerm : Coe (Subst.Action Term) Term where
+  coe := Term.from_action
 
 @[simp]
-def Surface.Term.rmap (lf : Endo Ren) (r : Ren) : Surface.Term -> Surface.Term
+def Term.rmap (r : Ren) : Term -> Term
 | `#x => `#(r x)
 | g`#x => g`#x
-| lamt A t => lamt A (rmap lf r t)
-| lam A t => lam A (rmap lf (lf r) t)
-| app t1 t2 => app (rmap lf r t1) (rmap lf r t2)
-| appt t1 t2 => appt (rmap lf r t1) t2
-| .match t1 t2 t3 t4 => .match (rmap lf r t1) (λ i => rmap lf r (t2 i)) (λ i => rmap lf r (t3 i)) (rmap lf r t4)
+| lamt A t => lamt A (rmap r t)
+| lam A t => lam A (rmap r.lift t)
+| app t1 t2 => app (rmap r t1) (rmap r t2)
+| appt t1 t2 => appt (rmap r t1) t2
+| .match t1 t2 t3 t4 => .match (rmap r t1) (rmap r <$> t2) (rmap r <$> t3) (rmap r t4)
 
-instance Surface.instRenMap_Term : RenMap Surface.Term where
-  rmap := Surface.Term.rmap
+instance instRenMap_Term : RenMap Term where
+  rmap := Term.rmap
 
 @[simp]
-def Surface.Term.Ty.smap (lf : Endo (Subst Surface.Ty)) (σ : Subst Surface.Ty) : Surface.Term -> Surface.Term
+def Term.Ty.smap (σ : Subst Ty) : Term -> Term
 | `#x => `#x
 | g`#x => g`#x
-| app t1 t2 => app (smap lf σ t1) (smap lf σ t2)
-| appt t1 t2 => appt (smap lf σ t1) t2[σ:_]
-| lamt A t => lamt A (smap lf (lf σ) t)
-| lam A t => lam A[σ:_] (smap lf σ t)
-| .match t1 t2 t3 t4  => .match (smap lf σ t1) (λ i => smap lf σ (t2 i)) (λ i => smap lf σ (t3 i)) (smap lf σ t4)
+| app t1 t2 => app (smap σ t1) (smap σ t2)
+| appt t1 t2 => appt (smap σ t1) t2[σ:_]
+| lamt A t => lamt A (smap σ.lift t)
+| lam A t => lam A[σ:_] (smap σ t)
+| .match t1 t2 t3 t4  => .match (smap σ t1) (λ i => smap σ (t2 i)) (λ i => smap σ (t3 i)) (smap σ t4)
 
-instance Surface.instSubstMap_TermTy : SubstMap Surface.Term Surface.Ty where
-  smap := Surface.Term.Ty.smap
+instance instSubstMap_TermTy : SubstMap Term Ty where
+  smap := Term.Ty.smap
 
 @[simp]
-def Surface.Term.smap (lf : Endo (Subst Term)) (σ : Subst Term) : Term -> Term
+def Term.smap (σ : Subst Term) : Term -> Term
 | `#x => σ x
 | g`#x => g`#x
-| app t1 t2 => app (smap lf σ t1) (smap lf σ t2)
-| appt t1 t2 => appt (smap lf σ t1) t2
-| lamt A t => lamt A (smap lf (σ ◾ +1@Surface.Ty) t)
-| lam A t => lam A (smap lf (lf σ) t)
-| .match t1 t2 t3 t4 => .match (smap lf σ t1) (λ i => smap lf σ (t2 i)) (λ i => smap lf σ (t3 i)) (smap lf σ t4)
+| app t1 t2 => app (smap σ t1) (smap σ t2)
+| appt t1 t2 => appt (smap σ t1) t2
+| lamt A t => lamt A (smap (σ ◾ +1@Ty) t)
+| lam A t => lam A (smap σ.lift t)
+| .match t1 t2 t3 t4 => .match (smap σ t1) (λ i => smap σ (t2 i)) (λ i => smap σ (t3 i)) (smap σ t4)
 
-instance Surface.instSubstMap_TermTerm : SubstMap Surface.Term Surface.Term where
-  smap := Surface.Term.smap
-
-@[simp]
-theorem Surface.Term.subst_var : (`#x)[σ:Term] = σ x := by
-  unfold Subst.apply; simp [SubstMap.smap]
+instance instSubstMap_TermTerm : SubstMap Term Term where
+  smap := Term.smap
 
 @[simp]
-theorem Surface.Term.subst_global : (g`#x)[σ:Term] = g`#x := by
-  unfold Subst.apply; simp [SubstMap.smap]
+theorem Term.subst_var : (`#x)[σ:Term] = σ x := by
+  simp [SubstMap.smap]
 
 @[simp]
-theorem Surface.Term.subst_app : (app t1 t2)[σ:Term] = app t1[σ:_] t2[σ:_] := by
-  simp [Subst.apply, SubstMap.smap]
+theorem Term.subst_global : (g`#x)[σ:Term] = g`#x := by
+  simp [SubstMap.smap]
 
 @[simp]
-theorem Surface.Term.subst_appt : (appt t1 t2)[σ:Term] = appt t1[σ:_] t2 := by
-  simp [Subst.apply, SubstMap.smap]
+theorem Term.subst_app : (app t1 t2)[σ:Term] = app t1[σ:_] t2[σ:_] := by
+  simp [SubstMap.smap]
 
 @[simp]
-theorem Surface.Term.subst_lamt : (lamt A t)[σ:Term] = lamt A t[σ ◾ +1@Surface.Ty:_] := by
-  simp [Subst.apply, SubstMap.smap]
+theorem Term.subst_appt : (appt t1 t2)[σ:Term] = appt t1[σ:_] t2 := by
+  simp [SubstMap.smap]
 
 @[simp]
-theorem Surface.Term.subst_lam : (lam A t)[σ:Term] = lam A t[σ.lift:_] := by
-  simp [Subst.apply, SubstMap.smap]
+theorem Term.subst_lamt : (lamt A t)[σ:Term] = lamt A t[σ ◾ +1@Ty:_] := by
+  simp [SubstMap.smap]
 
 @[simp]
-theorem Surface.Term.subst_match
+theorem Term.subst_lam : (lam A t)[σ:Term] = lam A t[σ.lift:_] := by
+  simp [SubstMap.smap]
+
+@[simp]
+theorem Term.subst_match
   : (matchˢ! t1 t2 t3 t4)[σ:Term] = matchˢ! t1[σ:_] (λ i => (t2 i)[σ:_]) (λ i => (t3 i)[σ:_]) (t4[σ:_])
 := by
-  simp [Subst.apply, SubstMap.smap]
+  simp [SubstMap.smap]
 
 @[simp]
-theorem Surface.Term.from_action_compose {x} {σ τ : Subst Term}
+theorem Term.from_action_compose {x} {σ τ : Subst Term}
   : (from_action (σ x))[τ] = from_action ((σ ∘ τ) x)
 := by
-  simp [Surface.Term.from_action, Subst.compose]
+  simp [Term.from_action, Subst.compose]
   generalize zdef : σ x = z
-  cases z <;> simp [Surface.Term.from_action]
+  cases z <;> simp [Term.from_action]
 
 @[simp]
-theorem Surface.Term.Ty.subst_var : (`#x)[σ:Surface.Ty] = `#x := by
-  unfold Subst.apply; simp [SubstMap.smap]
+theorem Term.Ty.subst_var : (`#x)[σ:Ty] = `#x := by
+  simp [SubstMap.smap]
 
 @[simp]
-theorem Surface.Term.Ty.subst_global : (g`#x)[σ:Surface.Ty] = g`#x := by
-  unfold Subst.apply; simp [SubstMap.smap]
+theorem Term.Ty.subst_global : (g`#x)[σ:Ty] = g`#x := by
+  simp [SubstMap.smap]
 
 @[simp]
-theorem Surface.Term.Ty.subst_app : (app t1 t2)[σ:Surface.Ty] = app t1[σ:_] t2[σ:_] := by
-  simp [Subst.apply, SubstMap.smap]
+theorem Term.Ty.subst_app : (app t1 t2)[σ:Ty] = app t1[σ:_] t2[σ:_] := by
+  simp [SubstMap.smap]
 @[simp]
-theorem Surface.Term.Ty.subst_appt : (appt t1 t2)[σ:Surface.Ty] = appt t1[σ:_] t2[σ:_] := by
-  simp [Subst.apply, SubstMap.smap]
+theorem Term.Ty.subst_appt : (appt t1 t2)[σ:Ty] = appt t1[σ:_] t2[σ:_] := by
+  simp [SubstMap.smap]
 
 @[simp]
-theorem Surface.Term.Ty.subst_lamt : (lamt A t)[σ:Ty] = lamt A t[σ.lift:_] := by
-  simp [Subst.apply, SubstMap.smap]
+theorem Term.Ty.subst_lamt : (lamt A t)[σ:Ty] = lamt A t[σ.lift:_] := by
+  simp [SubstMap.smap]
 
 @[simp]
-theorem Surface.Term.Ty.subst_lam : (lam A t)[σ:Ty] = lam A[σ:_] t[σ:_] := by
-  simp [Subst.apply, SubstMap.smap]
+theorem Term.Ty.subst_lam : (lam A t)[σ:Ty] = lam A[σ:_] t[σ:_] := by
+  simp [SubstMap.smap]
 
 @[simp]
-theorem Surface.Term.Ty.subst_match
+theorem Term.Ty.subst_match
   : (matchˢ! t1 ps t2 t3)[σ:Ty] = matchˢ! t1[σ:_] (λ i => (ps i)[σ:_]) (λ i => (t2 i)[σ:_]) t3[σ:_]
 := by
-  simp [Subst.apply, SubstMap.smap]
+  simp [SubstMap.smap]
 
-theorem Surface.Term.Ty.apply_id {t : Surface.Term} : t[+0:Surface.Ty] = t := by
+theorem Term.Ty.apply_id {t : Term} : t[+0:Ty] = t := by
   induction t
   all_goals (simp at * <;> try simp [*])
 
-instance Surface.instSubstMapId_Ty_TermTy : SubstMapId Surface.Term Surface.Ty where
-  apply_id := Surface.Term.Ty.apply_id
+instance instSubstMapId_Ty_TermTy : SubstMapId Term Ty where
+  apply_id := Term.Ty.apply_id
 
 @[simp]
-theorem Surface.Term.hcompose_var {σ : Subst Term} {τ : Subst Ty}
-  : (σ ◾ τ) x = (Surface.Term.from_action (σ x))[τ:Ty]
+theorem Term.hcompose_var {σ : Subst Term} {τ : Subst Ty}
+  : (σ ◾ τ) x = (Term.from_action (σ x))[τ:Ty]
 := by
-  simp [Subst.hcompose, Surface.Term.from_action]
+  simp [Subst.hcompose, Term.from_action]
   generalize zdef : σ x = z
   cases z <;> simp
 
-theorem Surface.Term.apply_stable (r : Ren) (σ : Subst Term)
-  : r.to = σ -> Ren.apply (T := Term) r = Subst.apply σ
-:= by subst_solve_stable Term, r, σ
+theorem Term.apply_stable (r : Ren) (σ : Subst Term)
+  : r = σ -> rmap r =  smap σ
+:= by subst_solve_stable r, σ
 
 
-instance Surface.instSubstMapStable_Term : SubstMapStable Surface.Term where
-  apply_stable := Surface.Term.apply_stable
+instance instSubstMapStable_Term : SubstMapStable Term where
+  apply_stable := Term.apply_stable
 
-theorem Surface.Term.apply_ren_commute {s : Surface.Term} (r : Ren) (τ : Subst Surface.Ty)
-  : s[r.to][τ:Surface.Ty] = s[τ:Surface.Ty][r.to]
+theorem Term.apply_ren_commute {s : Term} (r : Ren) (τ : Subst Ty)
+  : s[r.to][τ:Ty] = s[τ:Ty][r.to]
 := by
   induction s generalizing r τ <;> simp [Ren.to] at *
   all_goals try simp [*]
   case lam A t ih =>
     replace ih := ih r.lift
-    rw [Ren.to_lift (S := Surface.Term)] at ih; simp at ih
+    rw [Ren.to_lift] at ih; simp at ih
     apply ih
 
-instance Surface.instSubstMapRenCommute_Term : SubstMapRenCommute Surface.Term Surface.Ty where
-  apply_ren_commute := Surface.Term.apply_ren_commute
 
-theorem Surface.Term.Ty.apply_compose {s : Term} {σ τ : Subst Ty} : s[σ:Ty][τ:_] = s[σ ∘ τ:_] := by
-  subst_solve_compose Surface.Ty, s, σ, τ
 
-instance Surface.instSubstMapCompose_TermTy : SubstMapCompose Surface.Term Surface.Ty where
-  apply_compose := Surface.Term.Ty.apply_compose
+instance instSubstMapRenCommute_Term : SubstMapRenCommute Term Ty where
+  apply_ren_commute := Term.apply_ren_commute
 
-theorem Surface.Term.apply_hcompose {s : Surface.Term} {σ : Subst Surface.Term} {τ : Subst Surface.Ty}
+theorem Term.Ty.apply_compose {s : Term} {σ τ : Subst Ty} : s[σ:Ty][τ:_] = s[σ ∘ τ:_] := by
+  subst_solve_compose Ty, s, σ, τ
+
+instance instSubstMapCompose_TermTy : SubstMapCompose Term Ty where
+  apply_compose := Term.Ty.apply_compose
+
+theorem Term.apply_hcompose {s : Term} {σ : Subst Term} {τ : Subst Ty}
   : s[σ][τ:_] = s[τ:_][σ ◾ τ]
-:= by subst_solve_hcompose Surface.Term, Surface.Ty, s, σ, τ
+:= by subst_solve_hcompose Term, Ty, s, σ, τ
 
-instance Surface.instSubstMapHetCompose_TermTy : SubstMapHetCompose Surface.Term Surface.Ty where
-  apply_hcompose := Surface.Term.apply_hcompose
+instance instSubstMapHetCompose_TermTy : SubstMapHetCompose Term Ty where
+  apply_hcompose := Term.apply_hcompose
 
-theorem Surface.Term.apply_id {t : Term} : t[+0] = t := by subst_solve_id Term, Ty, t
+theorem Term.apply_id {t : Term} : t[+0] = t := by induction t; all_goals (simp at *; try simp [*])
 
-instance Surface.instSubstMapId_TermTy : SubstMapId Surface.Term Surface.Term where
-  apply_id := Surface.Term.apply_id
+instance instSubstMapId_TermTy : SubstMapId Term Term where
+  apply_id := Term.apply_id
 
-theorem Surface.Term.apply_compose {s : Surface.Term} {σ τ : Subst Term} : s[σ][τ] = s[σ ∘ τ] := by
+theorem Term.apply_compose {s : Term} {σ τ : Subst Term} : s[σ][τ] = s[σ ∘ τ] := by
   subst_solve_compose Term, s, σ, τ
 
-instance Surface.instSubstMapCompose_TermTerm : SubstMapCompose Surface.Term Surface.Term where
-  apply_compose := Surface.Term.apply_compose
+instance instSubstMapCompose_TermTerm : SubstMapCompose Term Term where
+  apply_compose := Term.apply_compose
 
-inductive Surface.IteratedSubst where
+inductive IteratedSubst where
 | nil : IteratedSubst
 | term : Subst Term -> IteratedSubst -> IteratedSubst
 | type : Subst Ty -> IteratedSubst -> IteratedSubst
 
-def Surface.Term.isubst (t : Surface.Term) : IteratedSubst -> Term
+def Term.isubst (t : Term) : IteratedSubst -> Term
 | .nil => t
 | .term σ tl => t[σ].isubst tl
 | .type σ tl => t[σ:Ty].isubst tl
+
+end Surface
