Surface/Global.lean
@@ -6,21 +6,21 @@ import Surface.Term
 open LeanSubst
 
 inductive Surface.Global : Type where
-| data : String -> Kind -> Vec (String × Ty) n -> Global
+| data : String -> Kind -> Vect n (String × Ty) -> Global
 -- | opent : String -> Kind -> Global
 -- | openm : String -> Ty -> Global
 -- | defn : String -> Ty -> Term -> Global
 -- | inst : String -> Term -> Global
 -- | instty : String -> Ty -> Global
 
-def Surface.Global.repr (p : Nat) : (a : Surface.Global) -> Std.Format
+def Surface.Global.repr (_ : Nat) : (a : Surface.Global) -> Std.Format
 | .data (n := n + 1) s K ctors =>
-  let ts : Vec Std.Format (n + 1) := λ i =>
+  let ts : Vect (n + 1) Std.Format := λ i =>
     let (ctorN, ctorTy) := ctors i
     Std.Format.nest 4 <| ctorN ++ " : " ++ Surface.Ty.repr max_prec ctorTy
 
   ".data " ++ s ++ " : " ++ Surface.Kind.repr max_prec K ++ Std.Format.line
-    ++ "v" ++ Std.Format.sbracket (Vec.fold (λ c acc => acc ++ ", " ++ Std.Format.line ++ c) Std.Format.nil ts)
+    ++ "v" ++ Std.Format.sbracket (ts.fold Std.Format.nil (λ c acc => acc ++ ", " ++ Std.Format.line ++ c))
 | .data s K _ =>
   ".data " ++ s ++ " : " ++ Surface.Kind.repr max_prec K
 -- | .opent n K => ".opent " ++ n ++ " " ++ K.repr max_prec
@@ -48,7 +48,7 @@ instance Surface.instRepr_Globals : Repr Surface.GlobalEnv where
   reprPrec a p := Globals.repr p a
 
 inductive Surface.Entry : Type where
-| data : String -> Kind -> Vec (String × Ty) n -> Entry
+| data : String -> Kind -> Vect n (String × Ty) -> Entry
 | ctor : String -> Nat -> Ty -> Entry
 | opent : String -> Kind -> Entry
 | openm : String -> Ty -> Entry
@@ -94,11 +94,11 @@ def Surface.Entry.type : Entry -> Option Ty
 def Surface.lookup (x : String) : GlobalEnv -> Option Entry
 | [] => none
 | .cons (.data (n := n) y K ctors) tl =>
-  let ctors' : Vec (Option Entry) n := λ i =>
+  let ctors' : Vect n (Option Entry) := λ i =>
     let (z, A) := ctors i
     if x == z then return .ctor z i A else none
   if x == y then return .data y K ctors
-  else Vec.fold Option.or (lookup x tl) ctors'
+  else Vect.fold (lookup x tl) Option.or ctors'
 -- | .cons (.opent y a) tl =>
 --   if x == y then return .opent y a else lookup x tl
 -- | .cons (.openm y a) tl =>
