Surface/Term/BEq.lean
@@ -1,7 +1,9 @@
 import Surface.Ty
 import Surface.Term.Definition
 
-def Surface.Term.beq : Term -> Term -> Bool
+namespace Surface
+
+def Term.beq : Term -> Term -> Bool
 | var x, var y => x == y
 | global x, global y => x == y
 | appt a1 b1, appt a2 b2 => beq a1 a2 && b1 == b2
@@ -10,30 +12,29 @@ def Surface.Term.beq : Term -> Term -> Bool
 | lam A1 t1, lam A2 t2 => A1 == A2 && beq t1 t2
 | .match (n := n1) a1 b1 c1 d1, .match (n := n2) a2 b2 c2 d2 =>
   if h : n1 = n2 then
-    let c : Vec Bool n1 := λ i => beq (c1 i) (c2 (by rw [h] at i; exact i))
-    let p : Vec Bool n1 := λ i => beq (b1 i) (b2 (by rw[h] at i; exact i))
-    beq a1 a2 && Vec.fold (·&&·) true c && Vec.fold (·&&·) true p && beq d1 d2
+    let c : Vect n1 Bool := λ i => beq (c1 i) (c2 (by rw[h] at i; exact i))
+    let p : Vect n1 Bool := λ i => beq (b1 i) (b2 (by rw[h] at i; exact i))
+    beq a1 a2 && Vect.fold true (·&&·) c && Vect.fold true (·&&·) p && beq d1 d2
   else false
 | _, _ => false
 
-instance Surface.instBEq_Term : BEq Surface.Term where
+instance instBEq_Term : BEq Term where
   beq := Term.beq
 
-instance Surface.instReflBEq_Term : ReflBEq Term where
+instance instReflBEq_Term : ReflBEq Term where
   rfl := by
-    intro a; induction a <;> simp [Surface.instBEq_Term, Surface.Term.beq] at *
+    intro a; induction a <;> simp [instBEq_Term, Term.beq] at *
     all_goals (repeat assumption)
     constructor; assumption; assumption
     case «match» ih1 ih2 ih3 ih4 =>
     constructor
     · constructor
       · constructor; assumption;
-        unfold Vec.fold;
+        unfold Vect.fold;
         case _ n _ _ _ _ =>
         induction n
         case _ => simp
         case _ n ih v1 v2 =>
-          simp;
         -- case _ => rfl
         -- case _ =>
         --   split; case _ h =>
@@ -44,7 +45,7 @@ instance Surface.instReflBEq_Term : ReflBEq Term where
       · sorry
     · assumption
 
-instance Surface.instLawfulBEq_Term : LawfulBEq Term where
+instance instLawfulBEq_Term : LawfulBEq Term where
   eq_of_beq := by
     intro a b; cases a <;> simp [instBEq_Term] at *
     all_goals (induction b <;>
@@ -54,3 +55,5 @@ instance Surface.instLawfulBEq_Term : LawfulBEq Term where
     sorry
     sorry
     sorry
+
+end Surface
