Translation.lean
@@ -1,2 +1,6 @@
 import Core.Ty
 import Surface.Ty
+
+import Translation.Ty
+import Translation.Term
+import Translation.Global
